Stlc/Value.lean
@@ -8,10 +8,9 @@ open Syntax
 @[mk_iff]
 inductive Value : Term → Prop
 | abs {x τ t} : Value t[λ x : τ, t]
-| true : Value t[true]
-| false : Value t[false]
+| bool {b} : Value (.bool b)
 
-attribute [simp] Value.abs Value.true Value.false
+attribute [simp] Value.abs Value.bool
 
 @[simp]
 lemma Value.var_not {x : String} : ¬Value t[xⱽ] := by
@@ -26,6 +25,6 @@ lemma Value.ite_not {t₁ t₂ t₃ : Term} : ¬Value t[if t₁ then t₂ else t
   rintro ⟨⟩
 
 instance : DecidablePred Value := fun t ↦
-  decidable_of_bool (t matches .true | .false | .abs ..) (by cases t <;> simp)
+  decidable_of_bool (t matches .bool _ | .abs ..) (by cases t <;> simp)
 
 end Stlc.Term
